ADDED:  - locales definitions

QKD/HOLCF/Automata/Automata.hs
@@ -1,0 +1,258 @@
+{-# LANGUAGE EmptyDataDecls, RankNTypes, ScopedTypeVariables #-}
+
+module Automata(Msg, Proc, Num, Transaction, Nat, Action, test_automaton)
+  where {
+
+import Prelude ((==), (/=), (<), (<=), (>=), (>), (+), (-), (*), (/), (**),
+  (>>=), (>>), (=<<), (&&), (||), (^), (^^), (.), ($), ($!), (++), (!!), Eq,
+  error, id, return, not, fst, snd, map, filter, concat, concatMap, reverse,
+  zip, null, takeWhile, dropWhile, all, any, Integer, negate, abs, divMod,
+  String, Bool(True, False), Maybe(Nothing, Just));
+import Data.Bits ((.&.), (.|.), (.^.));
+import qualified Prelude;
+import qualified Data.Bits;
+
+data Msg a = Prepare a | Yes | No | Commit | Abort | Ack;
+
+equal_msg :: forall a. (Eq a) => Msg a -> Msg a -> Bool;
+equal_msg Abort Ack = False;
+equal_msg Ack Abort = False;
+equal_msg Commit Ack = False;
+equal_msg Ack Commit = False;
+equal_msg Commit Abort = False;
+equal_msg Abort Commit = False;
+equal_msg No Ack = False;
+equal_msg Ack No = False;
+equal_msg No Abort = False;
+equal_msg Abort No = False;
+equal_msg No Commit = False;
+equal_msg Commit No = False;
+equal_msg Yes Ack = False;
+equal_msg Ack Yes = False;
+equal_msg Yes Abort = False;
+equal_msg Abort Yes = False;
+equal_msg Yes Commit = False;
+equal_msg Commit Yes = False;
+equal_msg Yes No = False;
+equal_msg No Yes = False;
+equal_msg (Prepare x1) Ack = False;
+equal_msg Ack (Prepare x1) = False;
+equal_msg (Prepare x1) Abort = False;
+equal_msg Abort (Prepare x1) = False;
+equal_msg (Prepare x1) Commit = False;
+equal_msg Commit (Prepare x1) = False;
+equal_msg (Prepare x1) No = False;
+equal_msg No (Prepare x1) = False;
+equal_msg (Prepare x1) Yes = False;
+equal_msg Yes (Prepare x1) = False;
+equal_msg (Prepare x1) (Prepare y1) = x1 == y1;
+equal_msg Ack Ack = True;
+equal_msg Abort Abort = True;
+equal_msg Commit Commit = True;
+equal_msg No No = True;
+equal_msg Yes Yes = True;
+
+instance (Eq a) => Eq (Msg a) where {
+  a == b = equal_msg a b;
+};
+
+data Proc = P0 | P1;
+
+equal_proc :: Proc -> Proc -> Bool;
+equal_proc P0 P1 = False;
+equal_proc P1 P0 = False;
+equal_proc P1 P1 = True;
+equal_proc P0 P0 = True;
+
+instance Eq Proc where {
+  a == b = equal_proc a b;
+};
+
+data Num = One | Bit0 Num | Bit1 Num;
+
+one_integer :: Integer;
+one_integer = (1 :: Integer);
+
+class One a where {
+  one :: a;
+};
+
+instance One Integer where {
+  one = one_integer;
+};
+
+class Plus a where {
+  plus :: a -> a -> a;
+};
+
+instance Plus Integer where {
+  plus = (\ a b -> a + b);
+};
+
+class Zero a where {
+  zero :: a;
+};
+
+instance Zero Integer where {
+  zero = (0 :: Integer);
+};
+
+class (Plus a) => Semigroup_add a where {
+};
+
+class (One a, Semigroup_add a) => Numeral a where {
+};
+
+instance Semigroup_add Integer where {
+};
+
+instance Numeral Integer where {
+};
+
+class Times a where {
+  times :: a -> a -> a;
+};
+
+class (One a, Times a) => Power a where {
+};
+
+instance Times Integer where {
+  times = (\ a b -> a * b);
+};
+
+instance Power Integer where {
+};
+
+class (Semigroup_add a) => Ab_semigroup_add a where {
+};
+
+class (Times a) => Semigroup_mult a where {
+};
+
+class (Ab_semigroup_add a, Semigroup_mult a) => Semiring a where {
+};
+
+instance Ab_semigroup_add Integer where {
+};
+
+instance Semigroup_mult Integer where {
+};
+
+instance Semiring Integer where {
+};
+
+class (Times a, Zero a) => Mult_zero a where {
+};
+
+instance Mult_zero Integer where {
+};
+
+class (Semigroup_add a, Zero a) => Monoid_add a where {
+};
+
+class (Ab_semigroup_add a, Monoid_add a) => Comm_monoid_add a where {
+};
+
+class (Comm_monoid_add a, Mult_zero a, Semiring a) => Semiring_0 a where {
+};
+
+instance Monoid_add Integer where {
+};
+
+instance Comm_monoid_add Integer where {
+};
+
+instance Semiring_0 Integer where {
+};
+
+class (Semigroup_mult a, Power a) => Monoid_mult a where {
+};
+
+class (Monoid_mult a, Numeral a, Semiring a) => Semiring_numeral a where {
+};
+
+class (One a, Zero a) => Zero_neq_one a where {
+};
+
+class (Semiring_numeral a, Semiring_0 a, Zero_neq_one a) => Semiring_1 a where {
+};
+
+instance Monoid_mult Integer where {
+};
+
+instance Semiring_numeral Integer where {
+};
+
+instance Zero_neq_one Integer where {
+};
+
+instance Semiring_1 Integer where {
+};
+
+data Transaction = T0;
+
+equal_transaction :: Transaction -> Transaction -> Bool;
+equal_transaction T0 T0 = True;
+
+instance Eq Transaction where {
+  a == b = equal_transaction a b;
+};
+
+data Nat = Zero_nat | Suc Nat;
+
+data Action a b = Start a | Send a a b | Receive a a b | Timeout a | Restart a;
+
+member :: forall a. (Eq a) => [a] -> a -> Bool;
+member [] y = False;
+member (x : xs) y = x == y || member xs y;
+
+length_tailrec :: forall a. [a] -> Nat -> Nat;
+length_tailrec [] n = n;
+length_tailrec (x : xs) n = length_tailrec xs (Suc n);
+
+exec_step ::
+  [(Proc, (Proc, Msg Transaction))] ->
+    Action Proc (Msg Transaction) -> Maybe [(Proc, (Proc, Msg Transaction))];
+exec_step ma (Send s r m) =
+  Just (if member ma (s, (r, m)) then ma else (s, (r, m)) : ma);
+exec_step ma (Receive s r m) =
+  (if member ma (s, (r, m)) then Just ma else Nothing);
+exec_step m (Start v) = Nothing;
+exec_step m (Timeout v) = Nothing;
+exec_step m (Restart v) = Nothing;
+
+exec_run ::
+  [Action Proc (Msg Transaction)] ->
+    [(Proc, (Proc, Msg Transaction))] ->
+      Maybe [(Proc, (Proc, Msg Transaction))];
+exec_run [] m = Just m;
+exec_run (a : asa) m = (case exec_step m a of {
+                         Nothing -> Nothing;
+                         Just aa -> exec_run asa aa;
+                       });
+
+size_list :: forall a. [a] -> Nat;
+size_list xs = length_tailrec xs Zero_nat;
+
+of_nat_aux :: forall a. (Semiring_1 a) => (a -> a) -> Nat -> a -> a;
+of_nat_aux inc Zero_nat i = i;
+of_nat_aux inc (Suc n) i = of_nat_aux inc n (inc i);
+
+of_nat :: forall a. (Semiring_1 a) => Nat -> a;
+of_nat n = of_nat_aux (\ i -> plus i one) n zero;
+
+integer_of_nat :: Nat -> Integer;
+integer_of_nat = of_nat;
+
+test_automaton :: Integer -> Integer;
+test_automaton n =
+  (case exec_run
+          [Send P0 P1 (Prepare T0), Receive P0 P1 (Prepare T0), Send P1 P0 Ack,
+            Receive P1 P0 Ack]
+          []
+    of {
+    Nothing -> (-1 :: Integer);
+    Just m -> integer_of_nat (size_list m);
+  });
+
+}
