QKD/HOLCF/Automata/Main.hs
@@ -1,0 +1,8 @@
+module Main where
+
+import Automata
+import qualified Prelude
+
+main :: Prelude.IO ()
+main = do
+    Prelude.print (test_automaton 0)
