QKD/HOLCF/ClientAutomaton/ClientAutomaton.hs
@@ -1,0 +1,51 @@
+{-# LANGUAGE EmptyDataDecls, RankNTypes, ScopedTypeVariables #-}
+
+module
+  ClientAutomaton(Exec_msg(..), Exec_action(..), Client_exec_state(..),
+                   initial_client, client_exec_step)
+  where {
+
+import Prelude ((==), (/=), (<), (<=), (>=), (>), (+), (-), (*), (/), (**),
+  (>>=), (>>), (=<<), (&&), (||), (^), (^^), (.), ($), ($!), (++), (!!), Eq,
+  error, id, return, not, fst, snd, map, filter, concat, concatMap, reverse,
+  zip, null, takeWhile, dropWhile, all, any, Integer, negate, abs, divMod,
+  String, Bool(True, False), Maybe(Nothing, Just));
+import Data.Bits ((.&.), (.|.), (.^.));
+import qualified Prelude;
+import qualified Data.Bits;
+
+class Ord a where {
+  less_eq :: a -> a -> Bool;
+  less :: a -> a -> Bool;
+};
+
+instance Ord Integer where {
+  less_eq = (\ a b -> a <= b);
+  less = (\ a b -> a < b);
+};
+
+data Exec_msg = CounterMsg Integer | Ping | Pong;
+
+data Exec_action = Receive Integer Exec_msg | UpdateCounter | PingServer
+  | ClientJoined Integer;
+
+data Client_exec_state = ClientState Integer Integer;
+
+max :: forall a. (Ord a) => a -> a -> a;
+max a b = (if less_eq a b then b else a);
+
+initial_client :: Integer -> Client_exec_state;
+initial_client server = ClientState (0 :: Integer) server;
+
+client_exec_step ::
+  Client_exec_state ->
+    Exec_action -> (Client_exec_state, [(Integer, Exec_msg)]);
+client_exec_step (ClientState ca s) (Receive uu (CounterMsg c)) =
+  (ClientState (max ca c) s, []);
+client_exec_step (ClientState c s) PingServer = (ClientState c s, [(s, Ping)]);
+client_exec_step s (Receive v Ping) = (s, []);
+client_exec_step s (Receive v Pong) = (s, []);
+client_exec_step s UpdateCounter = (s, []);
+client_exec_step s (ClientJoined v) = (s, []);
+
+}
