QKD/HOLCF/Fibonacci/Fibonacci.hs
@@ -1,0 +1,198 @@
+{-# LANGUAGE EmptyDataDecls, RankNTypes, ScopedTypeVariables #-}
+
+module Fibonacci(Nat, fib_int) where {
+
+import Prelude ((==), (/=), (<), (<=), (>=), (>), (+), (-), (*), (/), (**),
+  (>>=), (>>), (=<<), (&&), (||), (^), (^^), (.), ($), ($!), (++), (!!), Eq,
+  error, id, return, not, fst, snd, map, filter, concat, concatMap, reverse,
+  zip, null, takeWhile, dropWhile, all, any, Integer, negate, abs, divMod,
+  String, Bool(True, False), Maybe(Nothing, Just));
+import Data.Bits ((.&.), (.|.), (.^.));
+import qualified Prelude;
+import qualified Data.Bits;
+
+data Num = One | Bit0 Num | Bit1 Num;
+
+one_integer :: Integer;
+one_integer = (1 :: Integer);
+
+class One a where {
+  one :: a;
+};
+
+instance One Integer where {
+  one = one_integer;
+};
+
+class Plus a where {
+  plus :: a -> a -> a;
+};
+
+instance Plus Integer where {
+  plus = (\ a b -> a + b);
+};
+
+class Zero a where {
+  zero :: a;
+};
+
+instance Zero Integer where {
+  zero = (0 :: Integer);
+};
+
+class (Plus a) => Semigroup_add a where {
+};
+
+class (One a, Semigroup_add a) => Numeral a where {
+};
+
+instance Semigroup_add Integer where {
+};
+
+instance Numeral Integer where {
+};
+
+class Times a where {
+  times :: a -> a -> a;
+};
+
+class (One a, Times a) => Power a where {
+};
+
+instance Times Integer where {
+  times = (\ a b -> a * b);
+};
+
+instance Power Integer where {
+};
+
+class (Semigroup_add a) => Ab_semigroup_add a where {
+};
+
+class (Times a) => Semigroup_mult a where {
+};
+
+class (Ab_semigroup_add a, Semigroup_mult a) => Semiring a where {
+};
+
+instance Ab_semigroup_add Integer where {
+};
+
+instance Semigroup_mult Integer where {
+};
+
+instance Semiring Integer where {
+};
+
+class (Times a, Zero a) => Mult_zero a where {
+};
+
+instance Mult_zero Integer where {
+};
+
+class (Semigroup_add a, Zero a) => Monoid_add a where {
+};
+
+class (Ab_semigroup_add a, Monoid_add a) => Comm_monoid_add a where {
+};
+
+class (Comm_monoid_add a, Mult_zero a, Semiring a) => Semiring_0 a where {
+};
+
+instance Monoid_add Integer where {
+};
+
+instance Comm_monoid_add Integer where {
+};
+
+instance Semiring_0 Integer where {
+};
+
+class (Semigroup_mult a, Power a) => Monoid_mult a where {
+};
+
+class (Monoid_mult a, Numeral a, Semiring a) => Semiring_numeral a where {
+};
+
+class (One a, Zero a) => Zero_neq_one a where {
+};
+
+class (Semiring_numeral a, Semiring_0 a, Zero_neq_one a) => Semiring_1 a where {
+};
+
+instance Monoid_mult Integer where {
+};
+
+instance Semiring_numeral Integer where {
+};
+
+instance Zero_neq_one Integer where {
+};
+
+instance Semiring_1 Integer where {
+};
+
+data Nat = Zero_nat | Suc Nat;
+
+plus_nat :: Nat -> Nat -> Nat;
+plus_nat Zero_nat n = n;
+plus_nat (Suc m) n = plus_nat m (Suc n);
+
+one_nat :: Nat;
+one_nat = Suc Zero_nat;
+
+fib :: Nat -> Nat;
+fib Zero_nat = Zero_nat;
+fib (Suc Zero_nat) = one_nat;
+fib (Suc (Suc n)) = plus_nat (fib n) (fib (Suc n));
+
+apsnd :: forall a b c. (a -> b) -> (c, a) -> (c, b);
+apsnd f (x, y) = (x, f y);
+
+divmod_integer :: Integer -> Integer -> (Integer, Integer);
+divmod_integer k l =
+  (if k == (0 :: Integer) then ((0 :: Integer), (0 :: Integer))
+    else (if (0 :: Integer) < l
+           then (if (0 :: Integer) < k then divMod (abs k) (abs l)
+                  else (case divMod (abs k) (abs l) of {
+                         (r, s) ->
+                           (if s == (0 :: Integer)
+                             then (negate r, (0 :: Integer))
+                             else (negate r - (1 :: Integer), l - s));
+                       }))
+           else (if l == (0 :: Integer) then ((0 :: Integer), k)
+                  else apsnd negate
+                         (if k < (0 :: Integer) then divMod (abs k) (abs l)
+                           else (case divMod (abs k) (abs l) of {
+                                  (r, s) ->
+                                    (if s == (0 :: Integer)
+                                      then (negate r, (0 :: Integer))
+                                      else (negate r - (1 :: Integer),
+     negate l - s));
+                                })))));
+
+nat_of_integer :: Integer -> Nat;
+nat_of_integer k =
+  (if k <= (0 :: Integer) then Zero_nat
+    else (case divmod_integer k (2 :: Integer) of {
+           (l, j) ->
+             let {
+               la = nat_of_integer l;
+               lb = plus_nat la la;
+             } in (if j == (0 :: Integer) then lb else plus_nat lb one_nat);
+         }));
+
+of_nat_aux :: forall a. (Semiring_1 a) => (a -> a) -> Nat -> a -> a;
+of_nat_aux inc Zero_nat i = i;
+of_nat_aux inc (Suc n) i = of_nat_aux inc n (inc i);
+
+of_nat :: forall a. (Semiring_1 a) => Nat -> a;
+of_nat n = of_nat_aux (\ i -> plus i one) n zero;
+
+integer_of_nat :: Nat -> Integer;
+integer_of_nat = of_nat;
+
+fib_int :: Integer -> Integer;
+fib_int n = integer_of_nat (fib (nat_of_integer n));
+
+}
