QKD/HOLCF/ServerAutomaton/ServerAutomaton.hs
@@ -1,0 +1,46 @@
+{-# LANGUAGE EmptyDataDecls, RankNTypes, ScopedTypeVariables #-}
+
+module
+  ServerAutomaton(Num, Exec_msg(..), Exec_action(..), Server_exec_state(..),
+                   initial_server, server_exec_step)
+  where {
+
+import Prelude ((==), (/=), (<), (<=), (>=), (>), (+), (-), (*), (/), (**),
+  (>>=), (>>), (=<<), (&&), (||), (^), (^^), (.), ($), ($!), (++), (!!), Eq,
+  error, id, return, not, fst, snd, map, filter, concat, concatMap, reverse,
+  zip, null, takeWhile, dropWhile, all, any, Integer, negate, abs, divMod,
+  String, Bool(True, False), Maybe(Nothing, Just));
+import Data.Bits ((.&.), (.|.), (.^.));
+import qualified Prelude;
+import qualified Data.Bits;
+
+data Num = One | Bit0 Num | Bit1 Num;
+
+data Exec_msg = CounterMsg Integer | Ping | Pong;
+
+data Exec_action = Receive Integer Exec_msg | UpdateCounter | PingServer
+  | ClientJoined Integer;
+
+data Server_exec_state = ServerState Integer [Integer];
+
+generateMsgs :: [Integer] -> Exec_msg -> [(Integer, Exec_msg)];
+generateMsgs [] uu = [];
+generateMsgs (p : ps) msg = (p, msg) : generateMsgs ps msg;
+
+initial_server :: Server_exec_state;
+initial_server = ServerState (0 :: Integer) [];
+
+server_exec_step ::
+  Server_exec_state ->
+    Exec_action -> (Server_exec_state, [(Integer, Exec_msg)]);
+server_exec_step (ServerState c clients) UpdateCounter =
+  (ServerState (c + (1 :: Integer)) clients,
+    generateMsgs clients (CounterMsg (c + (1 :: Integer))));
+server_exec_step s (Receive client Ping) = (s, [(client, Pong)]);
+server_exec_step (ServerState c clients) (ClientJoined p) =
+  (ServerState c (p : clients), []);
+server_exec_step s (Receive v (CounterMsg vb)) = (s, []);
+server_exec_step s (Receive v Pong) = (s, []);
+server_exec_step s PingServer = (s, []);
+
+}
