QKD/HOLCF/Automata_Channel_IOA.thy
@@ -1,0 +1,58 @@
+theory Automata_Channel_IOA
+  imports Automata_IOA Automata_Datatypes
+begin
+
+locale DirectedChannel_IOA = 
+  fixes pid_sender:: 'proc
+    and pid_rcpt:: 'proc
+    and start:: "'state"
+    and add_msg:: "'state \<Rightarrow> msg \<Rightarrow> 'state"
+    and rmv_msg:: "'state \<Rightarrow> msg \<Rightarrow> 'state"
+    and can_send_msg:: "'state \<Rightarrow> msg \<Rightarrow> bool"
+begin
+
+abbreviation channel_asig where "channel_asig \<equiv> ({Send pid_sender pid_rcpt m | m. True}, {Receive pid_sender pid_rcpt m | m. True}, {})"
+
+abbreviation channel_trans where
+"channel_trans \<equiv> 
+    {(state, Send pid_sender pid_rcpt m, add_msg state m) | state m. True}
+  \<union> {(state, Receive pid_sender pid_rcpt m, rmv_msg state m) | state m. can_send_msg state m}"  
+
+end
+
+sublocale DirectedChannel_IOA < IOA 
+  "(channel_asig,
+   {start},
+   (channel_trans),
+   {},
+   {})"
+  rewrites asig_eq:"asig = channel_asig"
+      and starts_eq:"starts = {start}"
+      and trans_eq:"trans = channel_trans"
+      and wfair_eq:"wfair = {}"
+      and sfair_eq:"sfair = {}"
+  apply (unfold_locales)
+proof -
+  let ?ioa = "(channel_asig, {start}, channel_trans, {}, {})"
+  show "is_asig_of ?ioa"
+    unfolding is_asig_of_def asig_of_def is_asig_def asig_projections by auto
+  show "is_starts_of ?ioa"
+    unfolding is_starts_of_def starts_of_def by simp
+  show "is_trans_of ?ioa"
+    unfolding is_trans_of_def trans_of_def trans_def asig_projections apply auto
+    unfolding asig_projections actions_def asig_of_def by auto
+  show "input_enabled ?ioa"
+    unfolding input_enabled_def asig_projections asig_of_def trans_of_def by auto
+  show "asig_of ?ioa = channel_asig"
+    unfolding asig_of_def by simp
+  show "starts_of ?ioa = {start}"
+    unfolding starts_of_def by simp
+  show "trans_of ?ioa = channel_trans"
+    unfolding trans_of_def by simp
+  show "wfair_of ?ioa = {}"
+    unfolding wfair_of_def by simp
+  show "sfair_of ?ioa = {}"
+    unfolding sfair_of_def by simp
+qed
+
+end
