QKD/HOLCF/Automata_DIOA.thy
@@ -1,0 +1,72 @@
+theory Automata_DIOA
+  imports Automata_IOA
+begin
+
+datatype ('state, 'msg) ioa_state = IoaState (IoaState_curState: 'state) (IoaState_msgBuffer: "'msg set")
+
+locale DIOA = 
+  fixes pid:: 'proc
+    and ins:: "'action set"
+    and outs:: "'action set"
+    and ints:: "'action set"
+    and start:: "'state"
+    and stepf:: "'state \<Rightarrow> 'action \<Rightarrow> 'state \<times> ('proc \<times> 'msg) set"
+    and mk_msg:: "'action \<Rightarrow> ('proc \<times> 'proc \<times> 'msg) option"
+  assumes valid_sig: "is_asig (ins, outs, ints)"
+      and valid_outs: "\<And>a msg. mk_msg a = Some msg \<Longrightarrow> a \<in> outs"
+begin
+
+definition asig where "asig = (ins, outs, ints)"
+
+definition trans where
+"trans = 
+    {(IoaState state msgs, a, IoaState state' (msgs \<union> (\<lambda>msg. (pid, msg)) ` sent)) | state state' a msgs sent. (stepf state a = (state', sent)) \<and> a \<in> (ins \<union> ints)}
+  \<union> {(IoaState state msgs, a, IoaState state (msgs - {msg})) | state msgs a msg. msg \<in> msgs \<and> mk_msg a = Some msg}"
+
+definition dioa where "dioa = (asig, {IoaState start {}}, trans, {}, {})"
+
+lemma is_asig: "is_asig_of dioa"
+  using valid_sig unfolding dioa_def is_asig_of_def asig_def asig_of_def by simp
+
+lemma is_start: "is_starts_of dioa"
+  unfolding is_starts_of_def dioa_def starts_of_def by simp
+
+lemma is_trans:
+  "is_trans_of dioa"
+  unfolding is_trans_of_def trans_of_def DIOA_def dioa_def trans_def asig_projections apply auto
+  unfolding asig_def asig_projections actions_def asig_of_def apply auto
+  using valid_outs by blast
+
+lemma is_input_enabled:
+  "input_enabled dioa"
+  unfolding input_enabled_def DIOA_def asig_projections asig_of_def trans_of_def apply auto
+  unfolding dioa_def asig_def trans_def apply auto
+  by (metis ioa_state.exhaust surj_pair)
+
+lemma is_ioa:
+  shows "Automata.IOA dioa"
+  unfolding Automata.IOA_def
+  using is_asig is_start is_trans is_input_enabled by metis
+end
+
+sublocale DIOA < IOA
+  ins
+  outs
+  ints
+  "{IoaState start {}}"
+  trans
+  "{}"
+  "{}"
+proof
+  show "is_asig_of ((ins, outs, ints), {IoaState start {}}, local.trans, {}, {})"
+    by (metis asig_def is_asig dioa_def)
+  show "is_starts_of ((ins, outs, ints), {IoaState start {}}, local.trans, {}, {})"
+    by (metis asig_def dioa_def is_start)
+  show "is_trans_of ((ins, outs, ints), {IoaState start {}}, local.trans, {}, {})"
+    by (metis asig_def dioa_def is_trans)
+  show "input_enabled ((ins, outs, ints), {IoaState start {}}, local.trans, {}, {})"
+    by (metis asig_def dioa_def is_input_enabled)
+qed
+
+
+end
