QKD/HOLCF/Automata_Datatypes.thy
@@ -1,0 +1,18 @@
+theory Automata_Datatypes
+  imports Main
+begin
+
+datatype ('state, 'msg) ioa_state = IoaState (IoaState_curState: 'state) (IoaState_msgBuffer: "'msg set")
+
+datatype msg = CounterMsg nat | Ping | Pong
+
+datatype ('proc, 'msg) action = 
+  UpdateCount (UpdateCount_target: 'proc) | 
+  PingServer (PingServer_target: 'proc) |
+  ClientJoined (ClientJoined_target: 'proc) (ClientJoined_client: 'proc) |
+  Send (Send_sender: 'proc) (Send_rcpt: 'proc) (Send_msg: 'msg) | 
+  Receive (Receive_sender: 'proc) (Receive_rcpt: 'proc) (Receive_msg: 'msg)
+
+datatype 'proc sstate = Count (Count_clientIDs: "'proc set") (Count_curCounter: nat)
+datatype 'proc cstate = Count (Count_server: 'proc) (Count_curCount: nat)
+end
