QKD/HOLCF/Automata_Export_Test.thy
@@ -1,0 +1,89 @@
+theory Automata_Export_Test
+  imports Automata_Helper
+begin
+
+(* --- Datatypes --- *)
+datatype msg = CounterMsg nat | Ping | Pong
+
+datatype ('proc, 'msg) action = 
+  UpdateCount (UpdateCount_target: 'proc) | 
+  PingServer (PingServer_target: 'proc) |
+  ClientJoined (ClientJoined_target: 'proc) (ClientJoined_client: 'proc) |
+  Send (Send_sender: 'proc) (Send_rcpt: 'proc) (Send_msg: 'msg) | 
+  Receive (Receive_sender: 'proc) (Receive_rcpt: 'proc) (Receive_msg: 'msg)
+
+
+(* --- Server --- *)
+datatype 'proc sstate = Count (Count_clientIDs: "'proc set") (Count_curCounter: nat)
+datatype 'proc server_state = Buffer (server_state_curState: "'proc sstate") (server_state_msgBuffer: "('proc \<times> 'proc \<times> msg) set")
+
+fun server_step:: "'proc sstate \<Rightarrow> ('proc, msg) action \<Rightarrow> 'proc sstate \<times> ('proc \<times> msg) set" where
+  \<open>server_step (Count clients counter) (UpdateCount _) = (Count clients (counter + 1), {(client, CounterMsg (counter + 1)) | client. client \<in> clients})\<close> |
+  \<open>server_step (Count clients counter) (ClientJoined _ newClient) = (Count (clients \<union> {newClient}) counter, {})\<close> |
+  \<open>server_step state (Receive client _ Ping) = (state, {(client, Pong)})\<close> |
+  \<open>server_step state _ = (state, {})\<close>
+
+definition server_trans:: "'proc \<Rightarrow> ('proc server_state \<times> ('proc, msg) action \<times> 'proc server_state) set" where
+"server_trans pid =
+  {(Buffer s msgs, UpdateCount pid, Buffer s' (msgs \<union> ((\<lambda>msg. (pid, msg)) ` sent))) | s s' a msgs sent. (server_step s a = (s', sent)) \<and> (\<exists>sender. a = UpdateCount pid \<or> a = Receive sender pid Ping \<or> a = ClientJoined pid sender)}
+  \<union> {(Buffer s msgs, Send pid rcpt msg, Buffer s (msgs - {(pid,rcpt,msg)})) | s msgs rcpt msg. (pid,rcpt,msg) \<in> msgs}"
+
+definition server_asig :: "'proc \<Rightarrow> ('proc, msg) action signature" where
+"server_asig pid =
+ ({Receive q pid m | q m. True} \<union> {UpdateCount pid} \<union> {ClientJoined pid newClient | newClient. True},
+  {Send pid q m | q m. True},
+  {})"
+
+definition Server :: "'proc \<Rightarrow> 'proc set \<Rightarrow> (('proc, msg) action, 'proc server_state) ioa" where
+"Server pid clients = (server_asig pid, {Buffer (Count clients 0) {}}, server_trans pid, {}, {})"
+
+
+(* --- Client --- *)
+datatype 'proc cstate = Count (Count_server: 'proc) (Count_curCount: nat)
+datatype 'proc client_state = Buffer (client_state_curState: "'proc cstate") (client_state_msgBuffer: "('proc \<times> 'proc \<times> msg) set")
+
+fun client_step:: "'proc cstate \<Rightarrow> ('proc, msg) action \<Rightarrow> 'proc cstate \<times> ('proc \<times> msg) set" where
+  \<open>client_step (Count s t) (Receive _ _ (CounterMsg t')) = (Count s (max t t'), {})\<close> |
+  \<open>client_step (Count s t) (PingServer _) = (Count s t, {(s, Ping)})\<close> |
+  \<open>client_step state _ = (state, {})\<close>
+
+definition client_trans:: "'proc \<Rightarrow> ('proc client_state \<times> ('proc, msg) action \<times> 'proc client_state) set" where
+"client_trans pid =
+  {(Buffer s msgs, a, Buffer s' (msgs \<union> ((\<lambda>msg. (pid, msg)) ` sent))) | s a s' msgs sent. client_step s a = (s', sent) \<and> (\<exists>s t. a = Receive s pid (CounterMsg t))}
+  \<union> {(Buffer s msgs, Send pid rcpt msg, Buffer s (msgs - {(pid,rcpt,msg)})) | s msgs rcpt msg. (pid,rcpt,msg) \<in> msgs}"
+
+definition client_asig:: "'proc \<Rightarrow> ('proc, msg) action signature" where
+"client_asig pid =
+ ({Receive q pid m | q m. True} \<union> {PingServer pid},
+  {Send pid q m| q m. True},
+  {})"
+
+definition Client:: "'proc \<Rightarrow> 'proc \<Rightarrow> (('proc, msg) action, 'proc client_state) ioa" where
+"Client sid pid = (client_asig pid, {Buffer (Count sid 0) {}}, client_trans pid, {}, {})"
+
+definition Clients:: "'proc \<Rightarrow> 'proc set \<Rightarrow> (('proc, msg) action, 'proc \<Rightarrow> 'proc client_state) ioa" where
+"Clients sid clients = set_to_ioa clients (Client sid)"
+
+(* --- Channel --- *)
+type_synonym 'proc chan_state = "('proc \<times> 'proc \<times> msg) set"
+
+definition chan_trans :: "('proc chan_state \<times> ('proc, msg) action \<times> 'proc chan_state) set" where
+"chan_trans =
+  {(M, Send s r m, M \<union> {(s,r,m)}) | M s r m. True}
+  \<union> {(M, Receive s r m, M) | M s r m. (s,r,m) \<in> M}"
+
+definition chan_asig :: "('proc, msg) action signature" where
+"chan_asig =
+ ({Send s r m | s r m. True},
+  {Receive s r m | s r m. True},
+  {})"
+
+definition Channel :: "(('proc, msg) action, 'proc chan_state) ioa" where
+"Channel = (chan_asig, { {} }, chan_trans, {}, {})"
+
+
+(* --- System Composition --- *)
+definition System where
+"System server clients = ((Server server clients \<parallel> Channel) \<parallel> Clients server clients)"
+
+end
