QKD/HOLCF/Automata_Export_Test_Exec.thy
@@ -1,0 +1,73 @@
+theory Automata_Export_Test_Exec
+  imports
+    Automata_Export_Test
+    "HOL-Library.Code_Target_Int"
+begin
+
+type_synonym process = integer
+
+datatype exec_msg = CounterMsg (CounterMsg_curCounter: integer) | Ping | Pong
+
+datatype exec_action = 
+  Receive (Receive_sender: process) (Receive_msg: exec_msg) | 
+  UpdateCounter | 
+  PingServer |
+  ClientJoined (ClientJoined_newClient: process)
+
+(* ================================================================ *)
+(* Server implementation                                            *)
+(* ================================================================ *)
+
+datatype server_exec_state = ServerState (server_exec_state_curCounter: integer) (server_exec_state_clients: "process list")
+
+fun generateMsgs:: "process list \<Rightarrow> exec_msg \<Rightarrow> (process \<times> exec_msg) list" where
+"generateMsgs [] _ = []" |
+"generateMsgs (p#ps) msg = (p, msg)#(generateMsgs ps msg)"
+
+fun server_exec_step:: "server_exec_state \<Rightarrow> exec_action \<Rightarrow> server_exec_state \<times> (process \<times> exec_msg) list" where
+"server_exec_step (ServerState c clients) UpdateCounter = (ServerState (c + 1) clients, generateMsgs clients (CounterMsg (c + 1)))" |
+"server_exec_step s (Receive client Ping) = (s, [(client, Pong)])" |
+"server_exec_step (ServerState c clients) (ClientJoined p) = (ServerState c (p#clients), [])" |
+"server_exec_step s _ = (s, [])"
+
+definition initial_server:: "server_exec_state" where
+"initial_server = ServerState 0 []"
+
+
+export_code
+  server_exec_step
+  initial_server
+  ServerState
+  CounterMsg Ping Pong
+  Receive UpdateCounter PingServer ClientJoined
+in Haskell
+  module_name ServerAutomaton
+  file "ServerAutomaton"
+
+
+(* ================================================================ *)
+(* Client implementation                                            *)
+(* ================================================================ *)
+
+datatype client_exec_state = ClientState (ClientState_curCounter: integer) (ClientState_serverId: process)
+
+fun client_exec_step:: "client_exec_state \<Rightarrow> exec_action \<Rightarrow> client_exec_state \<times> (process \<times> exec_msg) list" where
+"client_exec_step (ClientState c s) (Receive _ (CounterMsg c')) = (ClientState (max c c') s, [])" |
+"client_exec_step (ClientState c s) PingServer = (ClientState c s, [(s,Ping)])" |
+"client_exec_step s _ = (s, [])"
+
+definition initial_client:: "process \<Rightarrow> client_exec_state" where
+"initial_client server = ClientState 0 server"
+
+
+export_code
+  client_exec_step
+  initial_client
+  ClientState
+  CounterMsg Ping Pong
+  Receive UpdateCounter PingServer ClientJoined
+in Haskell
+  module_name ClientAutomaton
+  file "ClientAutomaton"
+
+end
