QKD/HOLCF/Automata_IOA.thy
@@ -1,0 +1,37 @@
+theory Automata_IOA
+  imports Automata
+begin
+
+locale IOA =
+  fixes ioa' :: "('a, 's) ioa"
+  assumes is_asig_of: "is_asig_of ioa'"
+      and is_starts_of: "is_starts_of ioa'"
+      and is_trans_of: "is_trans_of ioa'"
+      and input_enabled: "input_enabled ioa'"
+begin
+
+abbreviation asig where
+  \<open>asig \<equiv> asig_of ioa'\<close>
+
+abbreviation starts where
+  \<open>starts \<equiv> starts_of ioa'\<close>
+
+abbreviation trans where
+  \<open>trans \<equiv> trans_of ioa'\<close>
+
+abbreviation wfair where
+  \<open>wfair \<equiv> wfair_of ioa'\<close>
+
+abbreviation sfair where
+  \<open>sfair \<equiv> sfair_of ioa'\<close>
+
+abbreviation ioa where
+  \<open>ioa \<equiv> ioa'\<close>
+
+lemma is_ioa: "Automata.IOA ioa'"
+  unfolding Automata.IOA_def 
+  using is_asig_of is_starts_of is_trans_of input_enabled by simp
+
+end
+
+end
