QKD/HOLCF/Automata_Network_DIOA.thy
@@ -1,0 +1,61 @@
+theory Automata_Network_DIOA
+  imports Automata_IOA Automata_Datatypes
+begin
+
+locale Network_DIOA = 
+  fixes pid:: 'proc
+    and ins:: "('proc, msg) action set"
+    and start:: "'state"
+    and stepf:: "'state \<Rightarrow> ('proc, msg) action \<Rightarrow> 'state \<times> ('proc \<times> msg) set"
+  assumes valid_ins: "\<forall>rcpt msg. Send pid rcpt msg \<notin> ins"
+begin
+
+abbreviation dioa_asig where "dioa_asig \<equiv> (ins \<union> {Receive q pid m |q m. True}, {Send pid q m |q m. True}, {})"
+
+abbreviation dioa_trans where
+"dioa_trans \<equiv> 
+    {(IoaState state msgs, a, IoaState state' (msgs \<union> (\<lambda>msg. (pid, msg)) ` sent)) | state state' a msgs sent. (stepf state a = (state', sent)) \<and> a \<in> ins \<union> {Receive q pid m |q m. True}}
+  \<union> {(IoaState state msgs, Send pid q msg, IoaState state (msgs - {(pid, q, msg)})) | state msgs q msg. (pid, q, msg) \<in> msgs}"
+
+lemma deterministic:
+  assumes s1_trans:"(s, a, s1) \<in> dioa_trans"
+    and s2_trans:"(s, a, s2) \<in> dioa_trans"
+  shows "s1 = s2"
+  using assms valid_ins by auto
+
+end
+
+sublocale Network_DIOA < IOA "(dioa_asig, {IoaState start {}}, dioa_trans, {}, {})"
+  rewrites asig_eq:"asig = dioa_asig"
+      and starts_eq:"starts = {IoaState start {}}"
+      and trans_eq:"trans = dioa_trans"
+      and wfair_eq:"wfair = {}"
+      and sfair_eq:"sfair = {}"
+  apply (unfold_locales)
+proof -
+  let ?ioa = "(dioa_asig, {IoaState start {}}, dioa_trans, {}, {})"
+  show "is_asig_of ?ioa"
+    using valid_ins unfolding is_asig_of_def asig_of_def is_asig_def apply simp
+    unfolding asig_projections by auto
+  show "is_starts_of ?ioa"
+    unfolding is_starts_of_def starts_of_def by simp
+  show "is_trans_of ?ioa"
+    unfolding is_trans_of_def trans_of_def IOA_def trans_def asig_projections apply auto
+    unfolding asig_projections actions_def asig_of_def by auto
+  show "input_enabled ?ioa"
+    unfolding input_enabled_def asig_inputs_def asig_of_def trans_of_def apply auto
+    unfolding trans_def apply (metis ioa_state.exhaust old.prod.exhaust)
+    by (metis ioa_state.exhaust old.prod.exhaust)
+  show "asig_of ?ioa = dioa_asig"
+    unfolding asig_of_def by simp
+  show "starts_of ?ioa = {IoaState start {}}"
+    unfolding starts_of_def by simp
+  show "trans_of ?ioa = dioa_trans"
+    unfolding trans_of_def by simp
+  show "wfair_of ?ioa = {}"
+    unfolding wfair_of_def by simp
+  show "sfair_of ?ioa = {}"
+    unfolding sfair_of_def by simp
+qed
+
+end
