QKD/HOLCF/Automata_Par_IOA.thy
@@ -1,0 +1,85 @@
+theory Automata_Par_IOA
+  imports Automata_IOA
+begin
+
+locale Par_IOA =
+  A: IOA A + 
+  B: IOA B
+  for A :: "('a, 's) ioa"
+    and B :: "('a, 't) ioa" +
+  assumes compatible: "compatible A B"
+begin
+
+abbreviation par_trans where
+  \<open>par_trans \<equiv> {tr.
+        let
+          s = fst tr;
+          a = fst (snd tr);
+          t = snd (snd tr)
+        in
+          (a \<in> act A \<or> a \<in> act B) \<and>
+          (if a \<in> act A then (fst s, a, fst t) \<in> trans_of A
+           else fst t = fst s) \<and>
+          (if a \<in> act B then (snd s, a, snd t) \<in> trans_of B
+           else snd t = snd s)}\<close>
+
+end
+
+sublocale Par_IOA < IOA "A \<parallel> B"
+  rewrites asig_eq:"asig = asig_comp (asig_of A) (asig_of B)"
+     and inp_eq:"inp (A \<parallel> B) = (inp A \<union> inp B) - (out A \<union> out B)"
+     and out_eq:"out (A \<parallel> B) = out A \<union> out B"
+     and int_eq:"int (A \<parallel> B) = int A \<union> int B"
+     and act_eq:"act (A \<parallel> B) = act A \<union> act B"
+     and starts_eq:"starts = {p. fst p \<in> starts_of A \<and> snd p \<in> starts_of B}"
+     and trans_eq:"trans = par_trans"
+     and wfair_eq:"wfair = wfair_of A \<union> wfair_of B"
+     and sfair_eq:"sfair = sfair_of A \<union> sfair_of B"
+  apply (unfold_locales)
+proof -
+  let ?ioa = "A \<parallel> B"
+  show "is_asig_of ?ioa"
+    using compatible A.is_asig_of B.is_asig_of 
+    unfolding is_asig_of_def compatible_def asig_of_def is_asig_def par_def apply simp
+    unfolding asig_comp_def asig_projections actions_def by auto
+  show "is_starts_of ?ioa"
+    using A.is_starts_of B.is_starts_of starts_of_par
+    unfolding is_starts_of_def apply auto
+  proof -
+    fix x :: 's and xa :: 't
+    assume a1: "xa \<in> starts_of B"
+    assume a2: "starts_of ?ioa = {}"
+    obtain bb :: "('a set \<times> 'a set \<times> 'a set) \<times> 't set \<times> ('t \<times> 'a \<times> 't) set \<times> 'a set set \<times> 'a set set \<Rightarrow> ('a set \<times> 'a set \<times> 'a set) \<times> 's set \<times> ('s \<times> 'a \<times> 's) set \<times> 'a set set \<times> 'a set set \<Rightarrow> 's \<times> 't \<Rightarrow> bool" where
+      f3: "\<forall>X0 x1 x2. bb X0 x1 x2 = (snd x2 \<in> starts_of X0 \<and> fst x2 \<in> starts_of x1)"
+      by moura
+    then have "\<forall>p pa. starts_of (pa \<parallel> p) = Collect (bb p pa)"
+      using starts_of_par by blast
+    then show False
+      using f3 a2 a1 by (metis (no_types) A.is_starts_of empty_Collect_eq ex_in_conv fst_eqD is_starts_of_def snd_eqD)
+  qed
+  show "is_trans_of ?ioa"
+    using A.is_trans_of B.is_trans_of trans_of_par by simp
+  show "input_enabled ?ioa"
+    using compatible A.input_enabled B.input_enabled input_enabled_par by blast
+  show "asig_of ?ioa = asig_comp A.asig B.asig"
+    unfolding asig_of_def par_def by simp
+  show "starts_of ?ioa = {p. fst p \<in> A.starts \<and> snd p \<in> B.starts}"
+    unfolding starts_of_def par_def by simp
+  show in':"inp ?ioa = inp A \<union> inp B - (out A \<union> out B)"
+    unfolding par_def asig_of_def asig_inputs_def asig_comp_def by simp
+  show out':"out ?ioa = out A \<union> out B"
+    unfolding par_def asig_of_def asig_outputs_def asig_comp_def by simp
+  show int':"int ?ioa = int A \<union> int B"
+    unfolding par_def asig_of_def asig_internals_def asig_comp_def by simp
+  show "act ?ioa = act A \<union> act B"
+    using in' out' int'
+    unfolding actions_def par_def asig_projections asig_comp_def by auto
+  show "trans_of ?ioa = par_trans"
+    unfolding par_def trans_of_def by simp
+  show "wfair_of ?ioa = A.wfair \<union> B.wfair"
+    unfolding par_def wfair_of_def by simp
+  show "sfair_of ?ioa = A.sfair \<union> B.sfair"
+    unfolding par_def sfair_of_def by simp
+qed
+
+end
