QKD/HOLCF/Automata_Set_Ext.thy
@@ -1,0 +1,124 @@
+theory Automata_Set_Ext
+  imports Automata
+begin
+
+definition family_inputs:: "'i set \<Rightarrow> ('i \<Rightarrow> ('a, 's) ioa) \<Rightarrow> 'a set" where
+"family_inputs I g = (\<Union>i\<in>I. inputs (asig_of (g i)))"
+
+definition family_outputs:: "'i set \<Rightarrow> ('i \<Rightarrow> ('a, 's) ioa) \<Rightarrow> 'a set" where
+"family_outputs I g = (\<Union>i\<in>I. outputs (asig_of (g i)))"
+
+definition family_internals:: "'i set \<Rightarrow> ('i \<Rightarrow> ('a, 's) ioa) \<Rightarrow> 'a set" where
+"family_internals I g = (\<Union>i\<in>I. internals (asig_of (g i)))"
+
+definition family_actions:: "'i set \<Rightarrow> ('i \<Rightarrow> ('a, 's) ioa) \<Rightarrow> 'a set" where
+"family_actions I g = (\<Union>i\<in>I. actions (asig_of (g i)))"
+
+definition family_asig:: "'i set \<Rightarrow> ('i \<Rightarrow> ('a, 's) ioa) \<Rightarrow> 'a signature" where
+"family_asig I g = ( family_inputs I g - family_outputs I g,
+                     family_outputs I g, 
+                     family_internals I g)"
+
+lemmas family = family_inputs_def family_outputs_def family_internals_def family_actions_def family_asig_def
+
+definition pairwise_compatible:: "'i set \<Rightarrow> ('i \<Rightarrow> ('a, 's) ioa) \<Rightarrow> bool" where
+"pairwise_compatible I g \<longleftrightarrow> (\<forall>i\<in>I. \<forall>j\<in>I. i \<noteq> j \<longrightarrow> compatible (g i) (g j))"
+
+(*Lynch's condition: action may only occur in finitely many components *)
+
+definition finite_action_participation:: "'i set \<Rightarrow> ('i \<Rightarrow> ('a, 's) ioa) \<Rightarrow> bool" where
+"finite_action_participation I g \<longleftrightarrow> (\<forall>a. finite {i \<in> I. a \<in> actions (asig_of (g i))})"
+
+definition lynch_compatible:: "'i set \<Rightarrow> ('i \<Rightarrow> ('a, 's) ioa) \<Rightarrow> bool" where
+"lynch_compatible I g \<longleftrightarrow> pairwise_compatible I g \<and> finite_action_participation I g"
+
+
+definition set_to_ioa:: "'i set \<Rightarrow> ('i \<Rightarrow> ('a, 's) ioa) \<Rightarrow> ('a, 'i \<Rightarrow> 's) ioa" where
+"set_to_ioa I g = (family_asig I g,
+                    {\<sigma>. \<forall>i\<in>I. \<sigma> i \<in> starts_of (g i)},
+                    {(\<sigma>, a, \<tau>).
+                      a \<in> family_actions I g \<and>
+                          (\<forall>i.
+                             if i \<in> I \<and> a \<in> actions (asig_of (g i))
+                             then (\<sigma> i, a, \<tau> i) \<in> trans_of (g i)
+                             else \<tau> i = \<sigma> i)},
+                    (\<Union>i\<in>I. wfair_of (g i)),
+                    (\<Union>i\<in>I. sfair_of (g i)))"
+
+
+
+
+section Lemmas
+
+lemma family_actions_asig [simp]:
+"actions (family_asig I g) = family_actions I g"
+  unfolding family_asig_def
+            family_inputs_def
+            family_outputs_def
+            family_internals_def
+            family_actions_def
+            actions_def
+            asig_inputs_def
+            asig_outputs_def
+            asig_internals_def
+  by auto
+
+lemma asig_of_set_ioa [simp]:
+"asig_of (set_to_ioa I g) = family_asig I g"
+  by (simp add: set_to_ioa_def ioa_projections)
+
+lemma starts_of_set_ioa [simp]:
+"starts_of (set_to_ioa I g) = {\<sigma>. \<forall>i\<in>I. \<sigma> i \<in> starts_of (g i)}"
+  by (simp add: set_to_ioa_def ioa_projections)
+
+lemma trans_of_set_ioa [simp]:
+"trans_of (set_to_ioa I g) =
+   {(\<sigma>, a, \<tau>).
+      a \<in> family_actions I g \<and>
+      (\<forall>i.
+         if i \<in> I \<and> a \<in> actions (asig_of (g i))
+         then (\<sigma> i, a, \<tau> i) \<in> trans_of (g i)
+         else \<tau> i = \<sigma> i)}"
+  by (simp add: set_to_ioa_def ioa_projections)
+
+lemma wfair_of_set_ioa [simp]:
+"wfair_of (set_to_ioa I g) = (\<Union>i\<in>I. wfair_of (g i))"
+  by (simp add: set_to_ioa_def ioa_projections)
+
+lemma sfair_of_set_ioa [simp]:
+"sfair_of (set_to_ioa I g) = (\<Union>i\<in>I. sfair_of (g i))"
+  by (simp add: set_to_ioa_def ioa_projections)
+
+lemma act_in_set_is_inp:
+  assumes compatible: "pairwise_compatible I g"
+    and valid_components: "\<And>i. i \<in> I \<Longrightarrow> IOA (g i)"
+    and a_inp: "a \<in> inputs (asig_of (set_to_ioa I g))"
+    and iI: "i \<in> I" 
+    and a_act: "a \<in> act (g i)"
+  shows "a \<in> inp (g i)"
+proof -
+  have "a \<notin> out (g i)"
+    using assms apply simp
+    unfolding asig_projections family_asig_def family_inputs_def family_outputs_def asig_of_def by auto
+  moreover have "a \<notin> int (g i)"
+    using assms compatible valid_components 
+    unfolding set_to_ioa_def family_asig_def family_inputs_def asig_projections apply auto
+    unfolding asig_of_def family_outputs_def family_inputs_def pairwise_compatible_def apply auto
+    unfolding asig_projections actions_def apply auto
+    unfolding compatible_def asig_projections asig_of_def actions_def apply auto
+    unfolding Automata.IOA_def is_asig_of_def is_asig_def asig_of_def asig_projections apply auto
+    unfolding input_enabled_def asig_projections trans_of_def asig_of_def is_trans_of_def apply auto
+    unfolding is_starts_of_def starts_of_def actions_def asig_projections apply auto
+    by (metis Int_iff inf_sup_absorb)
+  ultimately show "a \<in> inp (g i)"
+    using a_act unfolding actions_def by blast
+qed
+
+lemma set_trans_dest: 
+  assumes "(s, a, t) \<in> trans_of (set_to_ioa I g)"
+  shows "\<exists>i \<in> I. a \<in> act (g i)"
+  using assms
+  unfolding trans_of_def set_to_ioa_def apply simp
+  by (simp add: family_actions_def)
+
+end
