QKD/HOLCF/Automata_System_Def.thy
@@ -1,0 +1,197 @@
+theory Automata_System_Def
+  imports Automata_Network_DIOA Automata_Set_IOA Automata_Par_IOA Automata_Channel_IOA
+begin
+
+locale Global_Network =
+  fixes server :: "'proc"
+    and clients :: "'proc set"
+  assumes server_not_client: "server \<notin> clients"
+begin
+
+section Server
+
+fun server_step:: "'proc sstate \<Rightarrow> ('proc, msg) action \<Rightarrow> 'proc sstate \<times> ('proc \<times> msg) set" where
+  \<open>server_step (sstate.Count cls counter) (UpdateCount _) = (sstate.Count cls (counter + 1), {(client, CounterMsg (counter + 1)) | client. client \<in> cls})\<close> |
+  \<open>server_step (sstate.Count cls counter) (ClientJoined _ newClient) = (sstate.Count (cls \<union> {newClient}) counter, {})\<close> |
+  \<open>server_step state (Receive client _ Ping) = (state, {(client, Pong)})\<close> |
+  \<open>server_step state _ = (state, {})\<close>
+
+sublocale Server: Network_DIOA
+  server
+  "{UpdateCount server} \<union> {ClientJoined server newClient | newClient. True}"
+  "(sstate.Count clients 0)"
+  server_step
+proof
+  show "\<forall>rcpt msg. Send server rcpt msg \<notin> {UpdateCount server} \<union> {ClientJoined server newClient |newClient. True}"
+    by simp
+qed
+
+
+
+section Clients
+
+fun client_step:: "'proc cstate \<Rightarrow> ('proc, msg) action \<Rightarrow> 'proc cstate \<times> ('proc \<times> msg) set" where
+  \<open>client_step (cstate.Count s t) (Receive _ _ (CounterMsg t')) = (cstate.Count s (max t t'), {})\<close> |
+  \<open>client_step (cstate.Count s t) (PingServer _) = (cstate.Count s t, {(s, Ping)})\<close> |
+  \<open>client_step state _ = (state, {})\<close>
+
+sublocale Client: Network_DIOA
+  pid
+  "{PingServer pid}"
+  "(cstate.Count sid 0)"
+  client_step
+  for sid pid
+proof
+  show "\<forall>rcpt msg. Send pid rcpt msg \<notin> {PingServer pid}"
+    by simp
+qed
+
+sublocale Clients: Set_IOA
+  clients
+  "\<lambda>id. Client.ioa id server"
+  rewrites "int Clients.ioa = {}"
+  apply(unfold_locales)
+proof -
+  show "pairwise_compatible clients (\<lambda>id. Client.ioa id server)"
+    unfolding pairwise_compatible_def compatible_def asig_projections apply simp
+    unfolding asig_of_def by auto
+  show "\<And>i. i \<in> clients \<Longrightarrow> Automata.IOA (Client.ioa i server)"
+    using Client.is_ioa by simp
+  show "Automata.int (set_to_ioa clients (\<lambda>id. Client.ioa id server)) = {}"
+    sorry
+qed
+
+
+
+section Channels
+
+sublocale Fifo_Channel: DirectedChannel_IOA
+  pid_sender
+  pid_rcpt
+  "[]"
+  "\<lambda>msgs msg. msg#msgs"
+  "\<lambda>msgs msg. tl msgs"
+  "\<lambda>msgs msg. (if \<exists>x xs. msgs = x#xs then hd msgs = msg else False)"
+  for pid_sender pid_rcpt
+  done
+
+sublocale Lossy_Reorder_Channel: DirectedChannel_IOA
+  pid_sender  
+  pid_rcpt
+  "{}"
+  "\<lambda>s m. s \<union> {m}"
+  "\<lambda>s m. s"
+  "\<lambda>s m. m \<in> s"
+  for pid_sender pid_rcpt
+  done
+
+  (* 1. Server-to-Client Channels *)
+sublocale Channels_S2C: Set_IOA 
+  "{server} \<times> clients" 
+  "\<lambda>(src, dst). Fifo_Channel.ioa src dst"
+  rewrites inp_eq_s2c:"inp (set_to_ioa ({server} \<times> clients) (\<lambda>(src, dst). Fifo_Channel.ioa src dst))= {Send server r m| r m. r \<in> clients}"
+    and out_eq_s2c:"out (set_to_ioa ({server} \<times> clients) (\<lambda>(src, dst). Fifo_Channel.ioa src dst))= {Receive server r m| r m. r \<in> clients}"
+    and int_eq_s2c:"int (set_to_ioa ({server} \<times> clients) (\<lambda>(src, dst). Fifo_Channel.ioa src dst)) = {}"
+  apply (unfold_locales)
+proof -
+  show "pairwise_compatible ({server} \<times> clients) (\<lambda>(src, dst). Fifo_Channel.ioa src dst)" 
+    unfolding pairwise_compatible_def compatible_def apply auto
+    unfolding asig_projections asig_of_def apply simp
+      apply blast
+    by auto
+  show "\<And>i. i \<in> {server} \<times> clients \<Longrightarrow> Automata.IOA (case i of (src, dst) \<Rightarrow> Fifo_Channel.ioa src dst)"
+    by (metis (mono_tags, lifting) Fifo_Channel.IOA_axioms IOA.is_ioa case_prod_conv surj_pair)
+  show "inp (set_to_ioa ({server} \<times> clients) (\<lambda>(src, dst). Fifo_Channel.ioa src dst)) = {Send server r m |r m. r \<in> clients}"
+    unfolding asig_projections asig_of_def set_to_ioa_def family by force
+  show "out (set_to_ioa ({server} \<times> clients) (\<lambda>(src, dst). Fifo_Channel.ioa src dst)) = {Receive server r m |r m. r \<in> clients}"
+    unfolding asig_projections asig_of_def set_to_ioa_def family by force
+  show "int (set_to_ioa ({server} \<times> clients) (\<lambda>(src, dst). Fifo_Channel.ioa src dst)) = {}"
+    unfolding asig_projections asig_of_def set_to_ioa_def family by force
+qed
+
+  (* 2. Client-to-Server Channels *)
+sublocale Channels_C2S: Set_IOA
+  "clients \<times> {server}"
+  "\<lambda>(src, dst). Fifo_Channel.ioa src dst"
+  rewrites inp_eq_c2s:"inp (set_to_ioa (clients \<times> {server}) (\<lambda>(src, dst). Fifo_Channel.ioa src dst))= {Send s server m| s m. s \<in> clients}"
+    and out_eq_c2s:"out (set_to_ioa (clients \<times> {server}) (\<lambda>(src, dst). Fifo_Channel.ioa src dst))= {Receive s server m| s m. s \<in> clients}"
+    and int_eq_c2s:"int (set_to_ioa (clients \<times> {server}) (\<lambda>(src, dst). Fifo_Channel.ioa src dst)) = {}"
+  apply(unfold_locales)
+proof -
+  show "pairwise_compatible (clients \<times> {server}) (\<lambda>(src, dst). Fifo_Channel.ioa src dst)" 
+    unfolding pairwise_compatible_def compatible_def apply auto
+    unfolding asig_projections asig_of_def apply simp
+      apply blast
+    by auto  
+  show "\<And>i. i \<in> clients \<times> {server} \<Longrightarrow> Automata.IOA (case i of (src, dst) \<Rightarrow> Fifo_Channel.ioa src dst)" 
+    by (metis (mono_tags, lifting) Fifo_Channel.IOA_axioms IOA.is_ioa case_prod_conv surj_pair)
+  show "inp (set_to_ioa (clients \<times> {server}) (\<lambda>(src, dst). Fifo_Channel.ioa src dst))= {Send s server m| s m. s \<in> clients}"
+    unfolding asig_projections asig_of_def set_to_ioa_def family by force
+  show "out (set_to_ioa (clients \<times> {server}) (\<lambda>(src, dst). Fifo_Channel.ioa src dst))= {Receive s server m| s m. s \<in> clients}"
+    unfolding asig_projections asig_of_def set_to_ioa_def family by force
+  show "int (set_to_ioa (clients \<times> {server}) (\<lambda>(src, dst). Fifo_Channel.ioa src dst)) = {}"
+    unfolding asig_projections asig_of_def set_to_ioa_def family by force
+qed
+
+
+
+section Pars
+
+  (* 3. Compose Channels via Par_IOA *)
+sublocale Channels: Par_IOA 
+  "Channels_S2C.ioa"
+  "Channels_C2S.ioa"
+  rewrites inp_eq_cs:"inp (Channels_S2C.ioa \<parallel> Channels_C2S.ioa) = {Send s r m| s r m. (s \<in> clients \<and> r = server) \<or> (s = server \<and> r \<in> clients)}"
+    and out_eq_cs:"out (Channels_S2C.ioa \<parallel> Channels_C2S.ioa) = {Receive s r m| s r m. (s \<in> clients \<and> r = server) \<or> (s = server \<and> r \<in> clients)}"
+    and int_eq_cs:"int (Channels_S2C.ioa \<parallel> Channels_C2S.ioa) = {}"
+     apply (unfold_locales)
+proof -
+  show "compatible Channels_S2C.ioa Channels_C2S.ioa"
+    using server_not_client
+    unfolding compatible_def apply simp
+    unfolding asig_projections family asig_of_def by auto
+  show "inp (Channels_S2C.ioa \<parallel> Channels_C2S.ioa) = {Send s r m| s r m. (s \<in> clients \<and> r = server) \<or> (s = server \<and> r \<in> clients)}"
+    sorry
+  show "out (Channels_S2C.ioa \<parallel> Channels_C2S.ioa) = {Receive s r m| s r m. (s \<in> clients \<and> r = server) \<or> (s = server \<and> r \<in> clients)}"
+    sorry
+  show "int (Channels_S2C.ioa \<parallel> Channels_C2S.ioa) = {}"
+    sorry
+qed
+    
+    
+
+
+  (* 4. Compose Server with the Network Channels *)
+sublocale Server_Channels: Par_IOA 
+    "Server.ioa" 
+    "Channels.ioa"
+  proof unfold_locales
+    show "compatible Server.ioa Channels.ioa"
+      unfolding compatible_def asig_projections asig_of_def par_def apply simp
+      unfolding asig_comp_def set_to_ioa_def apply simp
+      unfolding asig_projections family apply simp
+      unfolding asig_of_def by auto
+  qed
+
+(* 5. Compose (Server + Channels) with the Clients to form the Final System *)
+sublocale System: Par_IOA 
+    "Server_Channels.ioa" 
+    "Clients.ioa"
+  proof unfold_locales
+    show "compatible Server_Channels.ioa Clients.ioa"
+      using server_not_client
+      unfolding compatible_def asig_projections asig_of_def par_def apply simp
+      unfolding asig_comp_def set_to_ioa_def apply simp
+      unfolding asig_projections family apply simp
+      unfolding asig_of_def by auto
+ qed
+
+definition System2 where
+  \<open>System2 \<equiv> (Server.ioa \<parallel> (Channels_S2C.ioa \<parallel> Channels_C2S.ioa)) \<parallel> Clients.ioa\<close>
+
+lemma "Automata.IOA System.ioa"
+  using System.is_ioa by simp
+
+end
+
+end
