QKD/HOLCF/Client_Imperative.thy
@@ -1,0 +1,83 @@
+theory Client_Imperative
+  imports
+    "HOL-Imperative_HOL.Ref"
+    "HOL-Library.Code_Target_Nat"
+begin
+
+
+section \<open>Message type\<close>
+
+datatype exec_msg =
+    Counter nat
+  | Ping
+  | Pong
+  | Stop
+
+
+section \<open>Imperative client state\<close>
+
+type_synonym client_state =
+  "nat ref \<times> bool ref"
+
+
+section \<open>Initial state\<close>
+
+definition initial_client :: "client_state Heap" where
+  "initial_client = do {
+      counter \<leftarrow> ref 0;
+      active \<leftarrow> ref False;
+      return (counter, active)
+   }"
+
+
+section \<open>Client transition\<close>
+
+fun client_step ::
+    "client_state \<Rightarrow> exec_msg \<Rightarrow> unit Heap"
+where
+
+  "client_step (counter, active) (Counter n) =
+      Ref.update counter n"
+
+| "client_step (counter, active) Ping =
+      Ref.update active True"
+
+| "client_step (counter, active) Pong =
+      Ref.update active False"
+
+| "client_step (counter, active) Stop =
+      return ()"
+
+
+section \<open>Observation functions\<close>
+
+definition client_counter ::
+    "client_state \<Rightarrow> nat Heap"
+where
+  "client_counter (counter, active) =
+      Ref.lookup counter"
+
+
+definition client_active ::
+    "client_state \<Rightarrow> bool Heap"
+where
+  "client_active (counter, active) =
+      Ref.lookup active"
+
+
+section \<open>Code export\<close>
+
+export_code
+    initial_client
+    client_step
+    client_counter
+    client_active
+    Counter
+    Ping
+    Pong
+    Stop
+  in Haskell
+  module_name ClientAutomaton
+  file "ClientAutomaton"
+
+end
